%
\documentclass[12pt]{article}
% geometry
\usepackage[left=1in,top=1in,right=1in,bottom=1in,letterpaper]{geometry}
\usepackage{listings}
%\usepackage{algorithm,algorithmic}
\usepackage{amssymb,amsmath}
\usepackage{dsfont}
\usepackage{url}
\usepackage[lined,ruled,linesnumbered]{algorithm2e}
\lstset{language=Python}          % Set your language (you can change the language for each code-block optionally)

\usepackage[usenames]{color}
\usepackage[color,final]{showkeys}
\definecolor{refkey}{gray}{0.8}
\definecolor{labelkey}{gray}{0.8}

\usepackage[normalem]{ulem}
\newcommand{\remove}[1]{{\color{Gray}\sout{#1}}}
\newcommand{\comm}[1]{{\color{red}(#1)}}
\newcommand{\revise}[1]{{\color{blue}#1}}


\usepackage[utf8]{inputenc}

% Default fixed font does not support bold face
\DeclareFixedFont{\ttb}{T1}{txtt}{bx}{n}{12} % for bold
\DeclareFixedFont{\ttm}{T1}{txtt}{m}{n}{12}  % for normal

% Custom colors
\usepackage{color}
\definecolor{deepblue}{rgb}{0,0,0.5}
\definecolor{deepred}{rgb}{0.6,0,0}
\definecolor{deepgreen}{rgb}{0,0.5,0}


\newtheorem{theorem}{Theorem}[section]
\newtheorem{corollary}{Corollary}[theorem]
\newtheorem{lemma}[theorem]{Lemma}


\newcommand{\xx}{{\bf x}}  
\newcommand{\bb}{{\bf b}} 
\newcommand{\ba}{{\bf a}} 
\newcommand{\bc}{{\bf c}} 
\newcommand{\ee}{{\bf e}} 
\newcommand{\ff}{{\bf f}} 
\newcommand{\nn}{{\bf n}} 
\newcommand{\rr}{{\bf r}} 
\newcommand{\uu}{{\bf u}} 
\newcommand{\vv}{{\bf v}} 
\newcommand{\FF}{{\bf F}} 
\newcommand{\bA}{{\bf A}} 
\newcommand{\bB}{{\bf B}} 
\newcommand{\bC}{{\bf C}} 
\newcommand{\bE}{{\bf E}} 
\newcommand{\bS}{{\bf S}} 
\newcommand{\bX}{{\bf X}} 
\newcommand{\bT}{{\bf T}} 


\newcommand{\bnabla}{{\bf \nabla}} 

\newcommand{\kk}{{\underline{\underline{k}}}} 
\newcommand{\cc}{{\underline{\underline c}}} 
\newcommand{\ssigma}{{\underline{\underline \sigma}}} 
\newcommand{\te}{{\underline{\underline e}}} 
\newcommand{\ta}{{\underline{\underline a}}} 

\newcommand{\RR}{{\mathbb R}}  
\newcommand{\EE}{{\mathbb E}}  

\newcommand{\GG}{{\mathcal G}}  
\newcommand{\LL}{{\mathcal L}} 
\newcommand{\UU}{{\mathcal U}} 
\newcommand{\cF}{{\mathcal F}} 

\newcommand{\dV}{{\text{d}V}} 
\newcommand{\dS}{{\text{d}S}} 

\newcommand{\Var}{\text{Var}}  
\newcommand{\std}{\text{std}}  

\newcommand{\pr}{{\partial}}  


\newcommand{\lambdat}{{\bf \lambda}}
\newcommand{\mx}[1]{\begin{pmatrix}#1\end{pmatrix}}
\newcommand{\dx}[1]{\text{ d}#1}


\begin{document}

\title{Math 272A Homework 1 Spring 2017}
\author{Chuyuan Fu}
\date{}

\maketitle

\section{Exercise 1}
\subsection{}
\begin{align*}
\bnabla\cdot(\phi\ba) &= \frac{\pr}{\pr x_i} (\phi a_i) \\
	&= \frac{\pr \phi}{\pr x_i} a_i + \phi\frac{\pr a_i}{\pr x_i} \\
	&= \ba \cdot \bnabla\phi +\phi \bnabla\cdot\ba
\end{align*}


\subsection{}
\begin{align*}
\bnabla\times(\phi\ba) &=\ee_i\epsilon_{ijk}\frac{\pr}{\pr x_j} (\phi a_k)\\
	 &=\ee_i\epsilon_{ijk} (\frac{\pr \phi}{\pr x_j}  a_k   + \phi \frac{\pr a_k}{\pr x_j})\\
	&= (\bnabla\phi)\times\ba +\phi \bnabla\times\ba
\end{align*}


\subsection{}
\begin{align*}
\bnabla\cdot(\bnabla\times\ba) &= \frac{\pr}{\pr x_i}(\epsilon_{ijk}\frac{\pr a_k}{\pr x_j} )\\
	&= \epsilon_{ijk}\frac{\pr^2 a_k}{\pr x_i\pr x_j}\\
	&= -\epsilon_{jik}\frac{\pr^2 a_k}{\pr x_i\pr x_j}\\
	&= -\epsilon_{jik}\frac{\pr^2 a_k}{\pr x_j\pr x_i}\\
	&= -\epsilon_{ijk}\frac{\pr^2 a_k}{\pr x_i\pr x_j}\\
	&=0
\end{align*}


\subsection{}
\begin{align*}
\bnabla\times(\bnabla\phi) &=  \ee_i\epsilon_{ijk}\frac{\pr}{\pr x_j} (\frac{\pr \phi}{\pr x_k})\\
 &=  - \ee_i\epsilon_{ikj}\frac{\pr}{\pr x_j} (\frac{\pr \phi}{\pr x_k})\\
 &= - \ee_i\epsilon_{ikj}\frac{\pr}{\pr x_k} (\frac{\pr \phi}{\pr x_j})\\
&= {\bf 0}
\end{align*}

\subsection{}
\begin{align*}
\bnabla\times(\ba\times\bb)&= \epsilon_{ijk} \frac{\pr}{\pr x_j} (\epsilon_{klm}a_lb_m)\\
	&=\epsilon_{kij}\epsilon_{klm} \frac{\pr}{\pr x_j} (a_lb_m)\\
	&= (\delta_{il}\delta_{jm} - \delta_{im}\delta_{jl}) (\frac{\pr a_l}{\pr x_j}b_m + a_l\frac{\pr b_m}{\pr x_j})\\
	&= \frac{\pr a_i}{\pr x_m}b_m  - \frac{\pr a_j}{\pr x_j}b_i + a_i\frac{\pr b_j}{\pr x_j} - a_j\frac{\pr b_i}{\pr x_j}\\
	&= \bb\cdot\bnabla\ba - \bb(\bnabla\cdot\ba) +  \ba(\bnabla\cdot\bb) - \ba\cdot\bnabla\bb
\end{align*}

\subsection{}
\begin{align*}
\bnabla\cdot(\ba\times\bb) &= \frac{\pr}{\pr x_i}(\epsilon_{ijk} a_jb_k)\\
		&= \epsilon_{ijk}  \frac{\pr a_j}{\pr x_i} b_k +  \epsilon_{ijk}  \frac{\pr b_k}{\pr x_i} a_j\\
		&= \epsilon_{kij}  \frac{\pr a_j}{\pr x_i} b_k -  \epsilon_{jik}  \frac{\pr b_k}{\pr x_i} a_j\\
		&= \bb\cdot(\bnabla\times\ba)  - \ba\cdot(\bnabla\times\bb)
\end{align*}


\subsection{}
\begin{align*}
\nabla\cdot(\ba\bb) &= \frac{\pr}{\pr x_i}a_ib_j \ee_j\\
	&= \frac{\pr a_i}{\pr x_i}b_j \ee_j +  a_i\frac{\pr b_j}{\pr x_i}\ee_j\\
	&= (\bnabla\cdot\ba)\bb + (\ba\cdot\bnabla)\bb
\end{align*}


\subsection{}
\begin{align*}
\bnabla\times(\bnabla\times\ba) &= \ee_i\epsilon_{ijk}\frac{\pr}{\pr x_j}\epsilon_{klm}\frac{\pr a_m}{\pr x_l}\\
&= \ee_i\epsilon_{kij}\epsilon_{klm}\frac{\pr^2 a_m}{\pr x_lx_j}\\
&= \ee_i(\delta_{il}\delta_{jm} - \delta_{im}\delta_{jl})\frac{\pr^2 a_m}{\pr x_lx_j}\\
&= \frac{\pr^2 a_j}{\pr x_ix_j}\ee_i - \frac{\pr^2 a_i}{\pr x_jx_j}\ee_i\\
&= \bnabla(\bnabla\cdot\ba) - \nabla^2\ba
\end{align*}

\section{Exercise 2}
\subsection{}
\begin{align*}
\int_S\nn\dx{S} &= \int_S\ee_i n_i\dx{S} \\
&=\int_V \ee_i\frac{\pr 1}{\pr x_i}\dx{V}\\
&= {\bf 0}
\end{align*}


\subsection{}
\begin{align*}
\int_S (\xx\times\ba)\times\nn\dx{S} &= \int_S\ee_i \epsilon_{ijk} (\epsilon_{jlm} x_la_m) n_k\dx{S}\\
	&=\int_S\ee_i \epsilon_{jki} \epsilon_{jlm} x_la_m n_k\dx{S}\\
	&=\int_S\ee_i (\delta_{kl}\delta_{im} - \delta_{km}\delta_{il}) x_la_mn_k\dx{S}\\
	&= \int_S\ee_i (x_ka_i - x_ia_k)n_k\dx{S}\\
	&= \int_V \ee_ia_i\frac{\pr x_k}{\pr x_k} - \ee_i\int \frac{\pr (x_ia_k)}{\partial x_k} \dx{V} \\
	&= \int_V 3\ba\dx{V} - \ee_i\int_V \delta_{ik}a_k \dx{V}\\
	& = 2V\ba
\end{align*}

\subsection{}
\begin{align*}
\int_C\phi\bnabla\phi\cdot\dx{\xx} &= \frac 1 2 \int_C\frac{\pr \phi^2}{\pr x_i}\dx{x_i}\\	
	&=0
\end{align*}

\section{Exercise 3}
\subsection{}
\[
\ba\bb\bc_{121} = 1 \quad \ba\bb\bc_{123} = 1 \quad  \ba\bb\bc_{221} = -1  \quad  \ba\bb\bc_{223} = -1
\]
\[
\ba\bb\bc_{131} = -1 \quad \ba\bb\bc_{133} = -1 \quad  \ba\bb\bc_{231} = 1  \quad  \ba\bb\bc_{233} = 1
\]

\subsection{}
\[
u_i' = l_{ik}u_k
\]
\[
x_j' = l_{jm}x_m
\]
\[
\Rightarrow\frac{\pr u_i'}{\pr x_j'} = l_{ik}\frac{\pr u_k}{\pr x_m}l_{jm} =  l_{ik}l_{jm} \frac{\pr u_k}{\pr x_m}
\]


\subsection{}
\[
\sigma_{ij}' = l_{ik}l_{jm}\sigma_{km}
\]
\[
x_j' = l_{jn}x_n
\]
\[
\Rightarrow\frac{\pr \sigma_{ij}' }{\pr x_j'} = l_{ik}l_{jm}l_{jn}\frac{\pr \sigma_{km}}{\pr x_n} = l_{ik}\delta_{mn}\frac{\sigma_{km}}{\pr x_n} = l_{ik}\frac{\sigma_{km}}{\pr x_m} 
\]

\subsection{}
\[
A_{ij}'  = l_{ik} l_{jl}A_{kl}
\]
\[
\Rightarrow A_{ii}' =   l_{ik} l_{il}A_{kl} = \delta_{kl} A_{kl} = A_{kk}
\]
\[
A_{ji}'  = l_{jm} l_{in}A_{mn}
\]
\[
\Rightarrow A_{ij}'A_{ji}' = l_{ik} l_{jl}A_{kl}l_{jm} l_{in}A_{mn} = \delta_{kn}\delta_{lm}A_{kl}A_{mn} = A_{nm}A_{mn}
\]















\end{document}


